Use diskset_pred in one spec

src/AtomicCp.v
@@ -130,16 +130,20 @@ Module ATOMICCP.
   Notation MSLL := BFILE.MSLL.
   Notation MSAlloc := BFILE.MSAlloc.
 
+  Definition temp_tree_pred Fm Ftop fsxp temp_fn tinum temp_tree ilist freelist mscs :=
+    (exists tfile' ilist' freelist',
+     let tree' := DIRTREE.update_subtree [temp_fn] (DIRTREE.TreeFile tinum tfile') temp_tree in
+     Fm * DIRTREE.rep fsxp Ftop tree' ilist' freelist' *
+     [[ DIRTREE.dirtree_safe ilist' (BFILE.pick_balloc freelist' (MSAlloc mscs)) tree'
+                              ilist  (BFILE.pick_balloc freelist  (MSAlloc mscs)) temp_tree ]]
+    )%pred.
+
   Theorem copydata_ok : forall fsxp src_inum tinum mscs,
     {< ds Fm Ftop temp_tree src_fn file tfile v0 t0 ilist freelist,
     PRE:hm
       LOG.rep (FSXPLog fsxp) (SB.rep fsxp) (LOG.NoTxn ds) (MSLL mscs) hm *
       [[[ ds!! ::: (Fm * DIRTREE.rep fsxp Ftop temp_tree ilist freelist) ]]] *
-      [[ forall d, d_in d ds -> exists tfile' ilist' freelist',
-         let tree' := DIRTREE.update_subtree [temp_fn] (DIRTREE.TreeFile tinum tfile') temp_tree in
-         DIRTREE.dirtree_safe ilist' (BFILE.pick_balloc freelist' (MSAlloc mscs)) tree'
-                              ilist  (BFILE.pick_balloc freelist  (MSAlloc mscs)) temp_tree /\
-         (Fm * DIRTREE.rep fsxp Ftop tree' ilist' freelist')%pred (list2nmem d) ]]%type *
+      [[ diskset_pred (temp_tree_pred Fm Ftop fsxp temp_fn tinum temp_tree ilist freelist mscs)  ds ]] *
       [[ DIRTREE.find_subtree [src_fn] temp_tree = Some (DIRTREE.TreeFile src_inum file) ]] *
       [[ DIRTREE.find_subtree [temp_fn] temp_tree = Some (DIRTREE.TreeFile tinum tfile) ]] *
       [[ src_fn <> temp_fn ]] *
